Test/civl/samples/ogcounter.bpl
@@ -1,7 +1,7 @@
 // RUN: %parallel-boogie "%s" > "%t"
 // RUN: %diff "%s.expect" "%t"
 
-type {:linear "tid"} X;
+type X;
 const MainTid: X;
 
 var {:layer 0,2} x: int;
@@ -23,15 +23,15 @@ left action {:layer 2} AtomicIncrBy2()
 modifies x;
 { x := x + 2; }
 
-yield procedure {:layer 2} EqualTo2({:linear "tid"} tid: X)
+yield procedure {:layer 2} EqualTo2({:linear} tid: One X)
 requires call YieldPre(tid);
 ensures call YieldPost();
 {
   call IncrBy2();
 }
 
-yield invariant {:layer 2} YieldPre({:linear "tid"} tid: X);
-invariant tid == MainTid && x == 0;
+yield invariant {:layer 2} YieldPre({:linear} tid: One X);
+invariant tid->val == MainTid && x == 0;
 
 yield invariant {:layer 2} YieldPost();
 invariant x == 2;
